move_to_next modified; cursor_has_next created; btree proofs moved to btree directory

verif/indices/ordered_interface.v
@@ -4,6 +4,8 @@ Require Import indices.unordered_flat.
 Require Import VST.floyd.library.
 Module OrderedIndex.
 
+(* ================= ORDERED INDEX DEFINITION =============== *)
+
 Record index :=
   {
     key: Type;
@@ -25,21 +27,18 @@ Record index :=
     cursor_repr: cursor -> val -> mpred;
     cursor_type: type;
 
-    (* helpers *)
-    valid_cursor: cursor -> bool;
-    norm: cursor -> cursor;
-
     (* props *)
+    cursor_has_next_props: cursor -> Prop;
     create_cursor_props: t -> val -> Prop;
     go_to_key_props: cursor -> Prop;
     move_to_next_props: cursor -> Prop;
-    move_to_previous_props: cursor -> Prop;
     move_to_first_props: cursor -> Prop;
-    move_to_last_props: cursor -> Prop;
     get_record_props: cursor -> Prop;
     put_record_props: cursor -> Prop;
 
     (* interface *)
+
+    cursor_has_next:  cursor -> bool;
 
     create_cursor: t -> cursor;
     create_index: t -> Prop;
@@ -50,11 +49,7 @@ Record index :=
 
     move_to_next: cursor -> cursor;
 
-    move_to_previous: cursor -> cursor;
-
     move_to_first: cursor -> cursor;
-
-    move_to_last: cursor -> cursor;
    
     get_record: cursor -> val;
 
@@ -63,8 +58,19 @@ Record index :=
   }.
 
 
+(* ================= ORDERED INDEX FUNSPECS =============== *)
 
-(* ================= VERIFIED =============== *)
+Definition cursor_has_next_spec 
+  (oi: OrderedIndex.index): funspec :=
+  WITH cur:oi.(cursor), pc:val
+  PRE [ tptr oi.(cursor_type) ]
+    PROP(oi.(cursor_has_next_props) cur)
+    PARAMS(pc) GLOBALS()
+    SEP(oi.(cursor_repr) cur pc)
+  POST [tint]
+    PROP()
+    LOCAL(temp ret_temp (Val.of_bool (oi.(cursor_has_next) cur)))
+    SEP(oi.(cursor_repr) cur pc).
 
 Definition go_to_key_spec 
   (oi: OrderedIndex.index): funspec :=
@@ -112,22 +118,10 @@ Definition move_to_next_spec
     PROP(oi.(move_to_next_props) cur)
     PARAMS(p) GLOBALS()
     SEP(oi.(cursor_repr) cur p)
-  POST [tvoid]
+  POST [tint]
     PROP()
-    LOCAL()
+    LOCAL(temp ret_temp (Val.of_bool (oi.(cursor_has_next) (oi.(move_to_next) cur))))
     SEP(oi.(cursor_repr) (oi.(move_to_next) cur) p).
-
-Definition move_to_previous_spec 
-  (oi: OrderedIndex.index): funspec :=
-  WITH p: val, cur: oi.(cursor)
-  PRE [ tptr oi.(cursor_type)]
-    PROP(oi.(move_to_previous_props) cur)
-    PARAMS(p) GLOBALS()
-    SEP(oi.(cursor_repr) cur p)
-  POST [tvoid]
-    PROP()
-    LOCAL()
-    SEP(oi.(cursor_repr) (oi.(move_to_previous) cur) p).
 
 Definition cardinality_spec 
   (oi: OrderedIndex.index): funspec :=
@@ -150,21 +144,9 @@ Definition move_to_first_spec
     SEP(mem_mgr gv; oi.(cursor_repr) cur p)
   POST [tint]
     PROP()
-    LOCAL(temp ret_temp (Val.of_bool (oi.(valid_cursor) (oi.(move_to_first) cur))))
+    LOCAL(temp ret_temp (Val.of_bool (oi.(cursor_has_next) (oi.(move_to_first) cur))))
     SEP(mem_mgr gv; oi.(cursor_repr) (oi.(move_to_first) cur) p).
-
-Definition move_to_last_spec 
-  (oi: OrderedIndex.index): funspec :=
-  WITH gv: globals, p: val, cur: oi.(cursor)
-  PRE [tptr oi.(cursor_type)]
-    PROP(oi.(move_to_last_props) cur)
-    PARAMS(p) GLOBALS()
-    SEP(mem_mgr gv; oi.(cursor_repr) cur p)
-  POST [tint]
-    PROP()
-    LOCAL(temp ret_temp (Val.of_bool (oi.(valid_cursor) (oi.(move_to_last) cur))))
-    SEP(mem_mgr gv; oi.(cursor_repr) (oi.(move_to_last) cur) p).
-
+ 
 Definition get_record_spec 
   (oi: OrderedIndex.index): funspec :=
   WITH p: val, cur: oi.(cursor)
@@ -173,9 +155,10 @@ Definition get_record_spec
     PARAMS(p) GLOBALS()
     SEP(oi.(cursor_repr) cur p)
   POST [tptr tvoid]
+    EX newc,
     PROP()
     LOCAL(temp ret_temp (oi.(get_record) cur))
-    SEP(oi.(cursor_repr) (oi.(norm) cur) p).
+    SEP(oi.(cursor_repr) newc p).
 
 Definition put_record_spec 
   (oi: OrderedIndex.index): funspec :=
