verif/indices/spec_BtreeIndexASI.v
@@ -14,25 +14,22 @@ Section BtreeIndexASI.
     (_RL_NewCursor, create_cursor_spec btree_index).
   Definition create_index_funspec := 
     (_RL_NewRelation, create_index_spec btree_index).
-  Definition move_to_next_funspec := 
-    (_RL_MoveToNext, move_to_next_spec btree_index).
-  Definition move_to_previous_funspec := 
-    (_RL_MoveToPrevious, move_to_previous_spec btree_index).
+  Definition cursor_has_next_funspec := 
+    (_RL_CursorIsValid, cursor_has_next_spec btree_index).
   Definition go_to_key_funspec :=
     (_goToKey, go_to_key_spec btree_index).
   Definition move_to_first_funspec :=
     (_RL_MoveToFirst, move_to_first_spec btree_index).
+  Definition move_to_next_funspec := 
+    (_RL_MoveToNextValid, move_to_next_spec btree_index).
   Definition get_record_funspec :=
     (_RL_GetRecord, get_record_spec btree_index).
   Definition put_record_funspec :=
     (_RL_PutRecord, put_record_spec btree_index).
 
-(* needs C fun 
-  Definition move_to_last_funspec. *)
-
   Definition BtreeIndexASI:funspecs := 
       [ cardinality_funspec; create_cursor_funspec; create_index_funspec; 
-        move_to_next_funspec; move_to_previous_funspec; go_to_key_funspec;
+        move_to_next_funspec; cursor_has_next_funspec; go_to_key_funspec;
         move_to_first_funspec; get_record_funspec; put_record_funspec].
 
 Definition BtreeIndex_exportedFunIDs :list ident := map fst BtreeIndexASI.
