verif/btrees/verif_movetonextvalid.v
@@ -1,0 +1,28 @@
+(** * verif_movetonextvalid.v : Correctness proof of RL_MoveToNextValid *)
+
+Require Import VST.floyd.proofauto.
+Require Import VST.floyd.library.
+Require Import relation_mem.
+Require Import VST.msl.wand_frame.
+Require Import VST.msl.iter_sepcon.
+Require Import VST.floyd.reassoc_seq.
+Require Import VST.floyd.field_at_wand.
+Require Import FunInd.
+Require Import btrees.
+Require Import btrees_sep.
+Require Import btrees_spec.
+Require Import verif_movetonext.
+
+Lemma body_RL_MoveToNextValid: semax_body Vprog Gprog f_RL_MoveToNextValid RL_MoveToNextValid_spec.
+Proof.
+  start_function.
+  forward_call(c, pc, r).
+  forward_call(r, (RL_MoveToNext c r), pc).
+  split3; auto. 
+  { destruct c.
+    { simpl. auto. }
+    { simpl. destruct p. simple_if_tac.
+      apply movetonext_complete. apply movetonext_complete. auto.
+      apply movetonext_complete. auto. }}
+  forward. entailer!. entailer!.
+Qed.
