verif/btrees/verif_numrecords.v
@@ -1,0 +1,31 @@
+Require Import VST.floyd.proofauto.
+Require Import VST.floyd.library.
+Require Import btrees.relation_mem.
+
+Require Import VST.msl.wand_frame.
+Require Import VST.msl.iter_sepcon.
+Require Import VST.floyd.reassoc_seq.
+Require Import VST.floyd.field_at_wand.
+Require Import FunInd.
+Require Import btrees.btrees.
+Require Import btrees.btrees_sep.
+Require Import btrees.btrees_spec.
+
+Lemma body_NumRecords: 
+  semax_body Vprog Gprog f_RL_NumRecords RL_NumRecords_spec.
+Proof. 
+  start_function. forward_if True.
+  { forward. entailer!. }
+  { assert_PROP(False). entailer!. contradiction. }
+  { unfold cursor_rep. Intros andc_end idx_end.
+    unfold relation_rep. destruct r as (n0, v). (* r = (n0, v) *)
+    Intros. forward. forward. forward. entailer!. 
+    { unfold relation_rep. cancel. unfold cursor_rep.
+      Exists andc_end idx_end. 
+      assert (K: Vlong (Int64.repr (get_numrec (n0, v))) = 
+                     Vptrofs (Ptrofs.repr (get_numrec (n0, v)))).
+      rewrite Vptrofs_unfold_true; auto.
+      rewrite ptrofs_to_int64_repr; auto.
+      rewrite K.
+      cancel. }}
+Qed.
