verif/indices/btree_instance.v
@@ -8,7 +8,6 @@ Require Import indices.btree_wrappers.
 
 Import OrderedIndex.
 
-
 Definition bt_relation := btrees.relation val.
 Definition bt_cursor := btrees.cursor val.
 
@@ -16,7 +15,6 @@ Definition put_record_rel (c: (bt_relation * bt_cursor)%type)
   (k: btrees.key) (v: btrees.V) (vptr: val) 
   (cnew: (bt_relation * bt_cursor)%type): Prop := 
 RL_PutRecord_rel (snd c) (fst c) k v vptr (fst cnew) (snd cnew).
-
 
 Definition btree_index : index :=
   {| key := btrees.key;
@@ -37,11 +35,10 @@ Definition btree_index : index :=
      cursor_repr := fun '(m, c) p => relation_rep m * cursor_rep c m p;
      cursor_type := tcursor;
 
-     (* helpers *)
-     valid_cursor := fun '(m, c) => isValid c m;
-     norm := fun '(m, c) => (m, normalize c m);
-
      (* Props *)
+    cursor_has_next_props := fun '(m, c) => 
+        complete_cursor c m /\ correct_depth m /\ root_wf (get_root m);
+
     create_cursor_props := fun m p => 
         snd m <> nullval /\ root_integrity (get_root m) /\ correct_depth m /\ getvalr m = p;
 
@@ -54,14 +51,6 @@ Definition btree_index : index :=
         correct_depth m /\ root_wf (get_root m) /\ 
         getval (get_root m) <> Vundef /\
         complete_cursor (moveToFirst (get_root m) c 0) m;
-
-    move_to_last_props := fun '(m, c) => (c = empty_cursor) /\
-        partial_cursor c m /\ root_integrity (get_root m) /\ 
-        correct_depth m /\
-        root_wf (get_root m) /\ 
-        complete_cursor (moveToLast val (get_root m) c 0) m;
-
-    move_to_previous_props := fun '(m, c) => complete_cursor c m;
 
     go_to_key_props := fun '(m, c) =>
         complete_cursor c m /\ correct_depth m /\ 
@@ -77,6 +66,7 @@ Definition btree_index : index :=
         get_numrec m < Int.max_signed - 1;
 
     (* interface *)
+     cursor_has_next := fun '(m, c) => isValid c m;
 
      cardinality := fun '(m, c) => get_numrec m;
 
@@ -86,8 +76,6 @@ Definition btree_index : index :=
 
      move_to_next := fun '(m, c) => (m, (RL_MoveToNext c m));
 
-     move_to_previous := fun '(m, c) => (m, (RL_MoveToPrevious c m));
-
      go_to_key := fun '(m, c) k => (m, goToKey c m k);
 
      move_to_first := fun '(m, c) =>  let (n, p) := m in (m, moveToFirst n empty_cursor O);
@@ -96,11 +84,56 @@ Definition btree_index : index :=
 
      put_record := put_record_rel;
 
-     (* needs C function *)
-     move_to_last := fun '(m, c) =>  let (n, p) := m in (m, moveToLast val n c (Zlength c));
-
    |}. 
 
+Lemma sub_cursor_has_next: funspec_sub (snd btrees_spec.RL_CursorIsValid_spec) 
+  (cursor_has_next_spec btree_index).
+Proof. 
+  do_funspec_sub. destruct w; simpl. destruct p; simpl.
+  simpl in H. Exists (b, b0, v) emp.
+  rewrite emp_sepcon.
+  apply andp_right.
+  { entailer!. }
+  { entailer!. simpl. entailer!. }
+Qed.
+
+Lemma sub_get_record: funspec_sub (snd btrees_spec.RL_GetRecord_spec) 
+  (get_record_spec btree_index).
+Proof. 
+  do_funspec_sub. destruct w; simpl. destruct p; simpl.
+  simpl in H. Exists (b, b0, v) emp.
+  rewrite emp_sepcon. 
+  apply andp_right.
+  { entailer!. }
+  { entailer!. entailer!. 
+    Exists (b, (normalize b0 b)).
+    entailer!. }
+Qed.
+
+Lemma sub_move_to_first: funspec_sub (snd btrees_spec.RL_MoveToFirst_spec)
+  (move_to_first_spec btree_index) .
+Proof. 
+  do_funspec_sub. destruct w; simpl. destruct p; simpl.
+  destruct p0; simpl. simpl in H. 
+  Exists (b, b0, v, (get_root b), g0) emp.
+  rewrite emp_sepcon.
+  apply andp_right.
+  { entailer!. }
+  { entailer!. entailer!; destruct b; simpl; try auto; try entailer!. }
+Qed.
+
+Lemma sub_move_to_next: funspec_sub (snd btrees_spec.RL_MoveToNextValid_spec)
+  (move_to_next_spec btree_index).
+Proof. 
+  do_funspec_sub. destruct w; simpl. 
+  destruct p; simpl.
+  simpl in H.
+  Exists (b0, v, b) emp.
+  rewrite emp_sepcon.
+  apply andp_right.
+  { entailer!. }
+  { entailer!. simpl. entailer!. }
+Qed.
 
 Lemma sub_cardinality: funspec_sub (snd btrees_spec.RL_NumRecords_spec)
 (cardinality_spec btree_index).
@@ -136,42 +169,6 @@ Proof.
     apply wand_frame_intro. }
 Qed.
 
-Lemma sub_get_record: funspec_sub (snd btrees_spec.RL_GetRecord_spec) 
-(get_record_spec btree_index).
-Proof. 
-  do_funspec_sub. destruct w; simpl. destruct p; simpl.
-  simpl in H. Exists (b, b0, v) emp.
-  rewrite emp_sepcon. 
-  apply andp_right.
-  { entailer!. }
-  { entailer!. entailer!. }
-Qed. 
-
-Lemma sub_move_to_first: funspec_sub (snd btrees_spec.RL_MoveToFirst_spec)
-  (move_to_first_spec btree_index) .
-Proof. 
-  do_funspec_sub. destruct w; simpl. destruct p; simpl.
-  destruct p0; simpl. simpl in H. 
-  Exists (b, b0, v, (get_root b), g0) emp.
-  rewrite emp_sepcon.
-  apply andp_right.
-  { entailer!. }
-  { entailer!. entailer!; destruct b; simpl; try auto; try entailer!. }
-Qed.
-
-Lemma sub_move_to_last: funspec_sub (btrees_spec.RL_MoveToLast_spec) 
-  (move_to_last_spec btree_index).
-Proof. 
-  do_funspec_sub. destruct w; simpl. destruct p; simpl.
-  destruct p0; simpl. simpl in H. 
-  Exists (b, b0, v, (get_root b), g0) emp.
-  rewrite emp_sepcon.
-  apply andp_right.
-  { entailer. }
-  { entailer!. entailer!; destruct b; simpl; try auto; try entailer!. 
-     unfold empty_cursor. rewrite Zlength_nil. cancel. }
-Qed.
-
 Lemma sub_go_to_key: funspec_sub (snd btrees_spec.goToKey_spec)
   (go_to_key_spec btree_index).
 Proof. 
@@ -180,32 +177,6 @@ Proof.
   do 3 destruct p; simpl.
   simpl in H.
   Exists (b0, v0, b, k) emp.
-  rewrite emp_sepcon.
-  apply andp_right.
-  { entailer!. }
-  { entailer!. }
-Qed.
-
-Lemma sub_move_to_next: funspec_sub (snd btrees_spec.RL_MoveToNext_spec)
-  (move_to_next_spec btree_index).
-Proof. 
-  do_funspec_sub. destruct w; simpl. 
-  destruct p; simpl.
-  simpl in H.
-  Exists (b0, v, b) emp.
-  rewrite emp_sepcon.
-  apply andp_right.
-  { entailer!. }
-  { entailer!. }
-Qed.
-
-Lemma sub_move_to_previous: funspec_sub (snd btrees_spec.RL_MoveToPrevious_spec)
-  (move_to_previous_spec btree_index).
-Proof. 
-  do_funspec_sub. destruct w; simpl. 
-  destruct p; simpl.
-  simpl in H.
-  Exists (b0, v, b) emp.
   rewrite emp_sepcon.
   apply andp_right.
   { entailer!. }
