verif/indices/btree_placeholders.v
@@ -1,0 +1,54 @@
+Require Import VST.floyd.proofauto.
+Require Import VST.floyd.library.
+Require Import btrees.relation_mem.
+
+Require Import VST.msl.wand_frame.
+Require Import VST.msl.iter_sepcon.
+Require Import VST.floyd.reassoc_seq.
+Require Import VST.floyd.field_at_wand.
+Require Import FunInd.
+Require Import btrees.btrees.
+Require Import btrees.btrees_sep.
+Require Import btrees.btrees_spec.
+
+Lemma body_RL_DeleteRelation: 
+  semax_body Vprog Gprog f_RL_DeleteRelation RL_DeleteRelation_spec.
+Proof. Admitted. 
+
+Lemma body_RL_DeleteRecord: 
+  semax_body Vprog Gprog f_RL_DeleteRecord RL_DeleteRecord_spec.
+Proof. Admitted.
+
+Lemma body_RL_FreeCursor: 
+  semax_body Vprog Gprog f_RL_FreeCursor RL_FreeCursor_spec.
+Proof. Admitted.
+
+Lemma body_RL_MoveToNextValid: 
+  semax_body Vprog Gprog f_RL_MoveToNextValid RL_MoveToNextValid_spec.
+Proof. Admitted.
+
+Lemma body_RL_MoveToPreviousNotFirst: 
+  semax_body Vprog Gprog f_RL_MoveToPreviousNotFirst RL_MoveToPreviousNotFirst_spec.
+Proof. Admitted.
+
+Lemma body_RL_PrintTree: 
+  semax_body Vprog Gprog f_RL_PrintTree RL_PrintTree_spec.
+Proof. Admitted.
+
+Lemma body_RL_PrintCursor: 
+  semax_body Vprog Gprog f_RL_PrintCursor RL_PrintCursor_spec.
+Proof. Admitted.
+
+Lemma body_handleDeleteBtree: 
+  semax_body Vprog Gprog f_handleDeleteBtree handleDeleteBtree_spec.
+Proof. Admitted.
+
+Lemma body_printTree: 
+  semax_body Vprog Gprog f_printTree printTree_spec.
+Proof. Admitted.
+
+Lemma body_printCursor: 
+  semax_body Vprog Gprog f_printCursor printCursor_spec.
+Proof. Admitted.
+
+
